combinatory completeness

PartialCombinatoryAlgebras/Basic.lean
@@ -1,12 +1,14 @@
 import Mathlib.Data.Part
 
+/-- A notation for definedness of a partial element. -/
+notation:50 u:max " ⇓ " => Part.Dom u
+
 /-- A partial binary operation on a set. -/
 class PartialApplication (A : Type*) where
   /-- partial application -/
   app : Part A → Part A → Part A
-
-/-- a partial element is defined, with explicit carrier -/
-notation:50 u:max " ⇓ " => Part.Dom u
+  strict_left : ∀ {u v : Part A}, (app u v) ⇓ → u ⇓
+  strict_right : ∀ {u v : Part A}, (app u v) ⇓ → v ⇓
 
 @[inherit_doc]
 infixl:70 (priority := high) " ⬝ " => PartialApplication.app
@@ -65,17 +67,22 @@ namespace Expr
   | .var x, η => .some (η x)
   | .app e₁ e₂, η => (eval e₁ η) ⬝ (eval e₂ η)
 
-  @[inherit_doc]
-  notation " ⟦" e "⟧ " η => Expr.eval e η
-
   def defined {Γ A} [PCA A] (e : Expr Γ A) :=
-    ∀ (η : Γ → A), (⟦ e ⟧ η) ⇓
+    ∀ (η : Γ → A), (eval e η) ⇓
+
+  def subst {Γ A} [PCA A] (a : A) : Expr (Extend Γ) A → Expr Γ A
+  | .K => .K
+  | .S => .S
+  | .elm b => .elm b
+  | .var .here => .elm a
+  | .var (.there x) => .var x
+  | .app e₁ e₂ => .app (subst a e₁) (subst a e₂)
 
   def abstr {Γ A} [PCA A] : Expr (Extend Γ) A → Expr Γ A
   | .K => .app .K .K
   | .S => .app .K .S
   | .elm a => .app (.K) (.elm a)
-  | .var (.here) => .app (.app .S .K) .K
+  | .var .here => .app (.app .S .K) .K
   | .var (.there x) => .app .K (.var x)
   | .app e₁ e₂ => .app (.app .S (abstr e₁)) (abstr e₂)
 
@@ -90,5 +97,34 @@ namespace Expr
       case here => simp [eval, PCA.defined_S₂, PCA.defined_S₁, PCA.defined_K₀]
       case there => simp [eval, PCA.defined_K₁]
     case app e₁ e₂ ih₁ ih₂ => simp [eval, PCA.defined_S₂, ih₁, ih₂]
+
+  lemma unnecessary_lemma {Γ A} [PCA A] (e : Expr (Extend Γ) A) :
+    ∀ (a : A) (η : Γ → A), eval (subst a e) η = eval e (extend η a) := by
+    intro a η
+    induction e
+    case K => simp [subst, eval]
+    case S => simp [subst, eval]
+    case elm => simp [subst, eval]
+    case var x =>
+      cases x
+      case here => simp [subst, eval, extend]
+      case there x => simp [subst, eval, extend]
+    case app e₁ e₂ ih₁ ih₂ => simp [subst, eval, ih₁, ih₂]
+
+  lemma eq_abstr {Γ A} [PCA A] (e : Expr (Extend Γ) A) :
+    ∀ (a : A) (η : Γ → A), eval (.app (abstr e) (.elm a)) η = eval e (extend η a) := by
+    intro a η
+    induction e
+    case K => simp [eval, PCA.eq_K, PCA.defined_K₀]
+    case S => simp [eval, PCA.eq_K, PCA.defined_S₀]
+    case elm => simp [eval, PCA.eq_K]
+    case var x =>
+      cases x
+      case here => simp [eval, extend, PCA.eq_S, PCA.eq_K, PCA.defined_K₀, PCA.defined_K₁]
+      case there x => simp [eval, extend, PCA.eq_K]
+    case app e₁ e₂ ih₁ ih₂ =>
+      simp [abstr, eval] at ih₁
+      simp [abstr, eval] at ih₂
+      simp [abstr, eval, PCA.eq_S, defined_abstr _ η, ih₁, ih₂]
 
 end Expr
